computation/computation_lib_extends2.v
@@ -1,0 +1,533 @@
+(*
+
+  Copyright 2014 Cornell University
+  Copyright 2015 Cornell University
+  Copyright 2016 Cornell University
+  Copyright 2017 Cornell University
+
+  This file is part of VPrl (the Verified Nuprl project).
+
+  VPrl is free software: you can redistribute it and/or modify
+  it under the terms of the GNU General Public License as published by
+  the Free Software Foundation, either version 3 of the License, or
+  (at your option) any later version.
+
+  VPrl is distributed in the hope that it will be useful,
+  but WITHOUT ANY WARRANTY; without even the implied warranty of
+  MERCHANTABILITY or FITNESS FOR A PARTICULAR PURPOSE.  See the
+  GNU General Public License for more details.
+
+  You should have received a copy of the GNU General Public License
+  along with VPrl.  If not, see <http://www.gnu.org/licenses/>.
+
+
+  Websites: http://nuprl.org/html/verification/
+            http://nuprl.org/html/Nuprl2Coq
+            https://github.com/vrahli/NuprlInCoq
+
+  Authors: Vincent Rahli
+
+ *)
+
+
+Require Export computation_lib_extends.
+Require Export computation_preserves_utok.
+
+
+Lemma nt_wf_oterm_snd {o} :
+  forall op l1 (t1 : @NTerm o) l2 t2 bs ,
+    nt_wf (oterm op (bterm l1 t1 :: bterm l2 t2 :: bs)) -> nt_wf t2.
+Proof.
+  introv w.
+  allrw @nt_wf_oterm_iff; repnd; allsimpl.
+  pose proof (w (bterm l2 t2)) as w1; autodimp w1 hyp.
+  allrw @bt_wf_iff; auto.
+Qed.
+Hint Resolve nt_wf_oterm_snd : slow.
+
+Hint Resolve nt_wf_oterm_fst : slow.
+
+Lemma lib_extends_implies_subset_get_utokens_lib {o} :
+  forall (lib1 lib2 : @library o) t,
+    lib_extends lib2 lib1
+    -> subset (get_utokens_lib lib1 t) (get_utokens_lib lib2 t).
+Proof.
+  introv ext i.
+  allrw in_app_iff; repndors; tcsp.
+  right.
+  eapply lib_extends_implies_subset_get_utokens_library; eauto.
+Qed.
+
+Lemma lib_extends_preserves_not_in_get_utokens_lib {o} :
+  forall (lib1 lib2 : @library o) t a,
+    lib_extends lib2 lib1
+    -> !LIn a (get_utokens_lib lib2 t)
+    -> !LIn a (get_utokens_lib lib1 t).
+Proof.
+  introv ext i j; destruct i.
+  eapply lib_extends_implies_subset_get_utokens_lib; eauto.
+Qed.
+Hint Resolve lib_extends_preserves_not_in_get_utokens_lib : slow.
+
+Hint Resolve subst_aux_preserves_wf : wf.
+
+Lemma subst_utokens_aux_var_ren_utok {o} :
+  forall (t : @NTerm o) a a' n,
+    (!LIn a' (get_utokens t) [+] a = a')
+    -> subst_utokens_aux (ren_utok t a a') [(a', mk_var n)]
+       = subst_utokens_aux t [(a, mk_var n)].
+Proof.
+  nterm_ind t as [v|f|op bs ind] Case; introv h; tcsp.
+  Case "oterm".
+  allrw @ren_utok_oterm.
+  allrw @subst_utokens_aux_oterm.
+
+  unfold ren_utok_op.
+  remember (get_utok op) as guo; symmetry in Heqguo; destruct guo; simpl.
+
+  - boolvar; subst; tcsp; simpl.
+
+    + unfold subst_utok; simpl; boolvar; tcsp.
+
+    + allrw; simpl.
+      unfold subst_utok; simpl.
+      boolvar; tcsp; subst; tcsp.
+
+      * repndors; tcsp.
+        apply not_in_get_utokens_implies_not_in_get_utokens_o in h.
+        apply get_utok_some_implies_get_utokens_o_eq in Heqguo.
+        rewrite Heqguo in h; simpl in h; allrw not_over_or; tcsp.
+
+      * allrw map_map; unfold compose.
+        f_equal.
+        apply eq_maps; introv i.
+        destruct x as [l t]; simpl.
+        f_equal.
+        eapply ind; eauto.
+        repndors; tcsp; eauto 3 with slow.
+
+  - allrw; simpl.
+    f_equal.
+    allrw map_map; unfold compose.
+    apply eq_maps; introv i.
+    destruct x as [l t]; simpl; f_equal.
+    eapply ind; eauto.
+    repndors; tcsp; eauto 3 with slow.
+Qed.
+
+Lemma subst_utokens_var_ren_utok {o} :
+  forall (t : @NTerm o) a a' n,
+    (!LIn a' (get_utokens t) [+] a = a')
+    -> subst_utokens (ren_utok t a a') [(a', mk_var n)]
+       = subst_utokens t [(a, mk_var n)].
+Proof.
+  introv h.
+  unfold subst_utokens; autorewrite with slow.
+  boolvar; tcsp.
+  - apply subst_utokens_aux_var_ren_utok; tcsp.
+  - rewrite change_bvars_alpha_ren_utok.
+    rewrite subst_utokens_aux_var_ren_utok; autorewrite with slow; tcsp.
+Qed.
+
+Lemma lib_extends_preserves_compute_step {o} :
+  forall (lib1 lib2 : library)
+         (ext  : lib_extends lib2 lib1) (* lib2 extends lib1 *)
+         (a b  : @NTerm o)
+         (wf   : nt_wf a)
+         (comp : compute_step lib1 a = csuccess b),
+    compute_step lib2 a = csuccess b.
+Proof.
+  nterm_ind1s a as [v|f ind|op bs ind] Case; introv wf comp.
+
+  - Case "vterm".
+    csunf comp; allsimpl; ginv.
+
+  - Case "sterm".
+    csunf comp; allsimpl; ginv.
+
+  - Case "oterm".
+    dopid op as [can|ncan|exc|abs] SCase.
+
+    + SCase "Can".
+      csunf comp; allsimpl; ginv.
+
+    + SCase "NCan".
+      destruct bs as [|b1 bs]; try (complete (allsimpl; ginv)).
+      destruct b1 as [l t]; try (complete (allsimpl; ginv)).
+      destruct l; try (complete (allsimpl; ginv)).
+
+      { destruct t as [x|f|op bts]; try (complete (allsimpl; ginv));[|].
+
+        - csunf comp; allsimpl.
+          dopid_noncan ncan SSCase; allsimpl; ginv.
+
+          SSCase "NEApply".
+
+          apply compute_step_eapply_success in comp; exrepnd; subst.
+          repndors; exrepnd; allsimpl; subst.
+
+          + apply compute_step_eapply2_success in comp1; repnd; subst.
+            repndors; exrepnd; subst; ginv.
+            csunf; simpl.
+            dcwf h; simpl.
+            boolvar; try omega.
+            rewrite Znat.Nat2Z.id; auto.
+
+          + csunf; simpl.
+            apply isexc_implies2 in comp0; exrepnd; subst.
+            dcwf h; simpl; auto.
+
+          + fold_terms.
+            rewrite compute_step_eapply_iscan_isnoncan_like; auto.
+            pose proof (ind arg2 arg2 []) as h; clear ind.
+            repeat (autodimp h hyp); eauto 3 with slow.
+            apply h in comp1; clear h; eauto 3 with slow.
+            SearchAbout nt_wf oterm.
+            rewrite comp1; auto.
+
+        - dopid op as [can2|ncan2|exc2|abs2] SSCase.
+
+          + SSCase "Can".
+            dopid_noncan ncan SSSCase.
+
+            {
+              SSSCase "NApply".
+
+              csunf comp; allsimpl.
+              apply compute_step_apply_success in comp.
+              repndors; exrepnd; subst; auto.
+            }
+
+            {
+              SSSCase "NEApply".
+
+              csunf comp; allsimpl.
+              apply compute_step_eapply_success in comp.
+              repndors; exrepnd; subst; auto.
+              repndors; exrepnd; subst; allsimpl; auto.
+
+              - apply compute_step_eapply2_success in comp1; repnd; subst.
+                repndors; exrepnd; subst; auto; ginv.
+
+                + unfold mk_lam in *; ginv.
+                  csunf; simpl.
+                  dcwf h; simpl.
+                  apply iscan_implies in comp0; repndors; exrepnd; subst; simpl; auto.
+
+                + unfold mk_nseq in *; allsimpl; ginv.
+                  csunf; simpl.
+                  dcwf h; simpl.
+                  boolvar; simpl; auto; try omega.
+                  rewrite Znat.Nat2Z.id; auto.
+
+                + unfold mk_choice_seq in *; allsimpl; ginv.
+                  csunf; simpl.
+                  dcwf h; simpl.
+                  boolvar; simpl; try omega.
+                  autorewrite with slow.
+                  eapply lib_extends_preserves_find_cs_value_at in comp5;[|eauto].
+                  allrw; auto.
+
+              - fold_terms; rewrite compute_step_eapply_iscan_isexc; auto.
+
+              - fold_terms; rewrite compute_step_eapply_iscan_isnoncan_like; auto.
+
+                pose proof (ind arg2 arg2 []) as q; clear ind.
+                repeat (autodimp q hyp); eauto 2 with slow.
+                apply q in comp1; clear q; eauto 2 with slow.
+                rewrite comp1; auto.
+            }
+
+            {
+              SSSCase "NFix".
+
+              csunf comp; allsimpl.
+              apply compute_step_fix_success in comp.
+              repndors; exrepnd; subst; auto.
+            }
+
+            {
+              SSSCase "NSpread".
+
+              csunf comp; allsimpl.
+              apply compute_step_spread_success in comp.
+              repndors; exrepnd; subst; auto.
+            }
+
+            {
+              SSSCase "NDsup".
+
+              csunf comp; allsimpl.
+              apply compute_step_dsup_success in comp.
+              repndors; exrepnd; subst; auto.
+            }
+
+            {
+              SSSCase "NDecide".
+
+              csunf comp; allsimpl.
+              apply compute_step_decide_success in comp.
+              repndors; exrepnd; subst; auto.
+              repndors; exrepnd; subst; auto.
+            }
+
+            {
+              SSSCase "NCbv".
+
+              csunf comp; allsimpl.
+              apply compute_step_cbv_success in comp.
+              repndors; exrepnd; subst; auto.
+            }
+
+            {
+              SSSCase "NSleep".
+
+              csunf comp; allsimpl.
+              apply compute_step_sleep_success in comp.
+              repndors; exrepnd; subst; auto.
+            }
+
+            {
+              SSSCase "NTUni".
+
+              csunf comp; allsimpl.
+              apply compute_step_tuni_success in comp.
+              repndors; exrepnd; subst; auto.
+              csunf; simpl.
+              unfold compute_step_tuni; simpl.
+              boolvar; try omega.
+              rewrite Znat.Nat2Z.id; auto.
+            }
+
+            {
+              SSSCase "NMinus".
+
+              csunf comp; allsimpl.
+              apply compute_step_minus_success in comp.
+              repndors; exrepnd; subst; auto.
+            }
+
+            {
+              SSSCase "NFresh".
+
+              csunf comp; allsimpl; ginv.
+            }
+
+            {
+              SSSCase "NTryCatch".
+
+              csunf comp; allsimpl.
+              apply compute_step_try_success in comp.
+              repndors; exrepnd; subst; auto.
+            }
+
+            {
+              SSSCase "NParallel".
+
+              csunf comp; allsimpl.
+              apply compute_step_parallel_success in comp.
+              repndors; exrepnd; subst; auto.
+            }
+
+            {
+              SSSCase "NCompOp".
+
+              apply compute_step_ncompop_can1_success in comp; repnd.
+              repndors; exrepnd; allsimpl; subst; tcsp.
+
+              - csunf; simpl.
+                dcwf h.
+
+              - rewrite compute_step_ncompop_ncanlike2; auto.
+                dcwf h.
+                pose proof (ind t t []) as q; clear ind.
+                repeat (autodimp q hyp); eauto 2 with slow.
+                apply q in comp4; clear q; eauto 2 with slow.
+                rewrite comp4; auto.
+
+              - csunf; simpl.
+                apply isexc_implies2 in comp1; exrepnd; subst.
+                dcwf h; simpl; auto.
+            }
+
+            {
+              SSSCase "NArithOp".
+
+              apply compute_step_narithop_can1_success in comp; repnd.
+              repndors; exrepnd; allsimpl; subst; tcsp.
+
+              - csunf; simpl.
+                dcwf h.
+
+              - rewrite compute_step_narithop_ncanlike2; auto.
+                dcwf h.
+                pose proof (ind t t []) as q; clear ind.
+                repeat (autodimp q hyp); eauto 2 with slow.
+                apply q in comp4; clear q; eauto 2 with slow.
+                rewrite comp4; auto.
+
+              - csunf; simpl.
+                apply isexc_implies2 in comp1; exrepnd; subst.
+                dcwf h; simpl; auto.
+            }
+
+            {
+              SSSCase "NCanTest".
+
+              csunf comp; allsimpl.
+              apply compute_step_can_test_success in comp.
+              repndors; exrepnd; subst; auto.
+            }
+
+          + SSCase "NCan".
+
+            csunf comp; allsimpl.
+            remember (compute_step lib1 (oterm (NCan ncan2) bts)) as c.
+            destruct c; allsimpl; ginv.
+            symmetry in Heqc.
+
+            pose proof (ind (oterm (NCan ncan2) bts) (oterm (NCan ncan2) bts) []) as q; clear ind.
+            repeat (autodimp q hyp); eauto 2 with slow.
+            apply q in Heqc; clear q; eauto 2 with slow.
+            csunf; simpl.
+            rewrite Heqc; auto.
+
+          + SSCase "Exc".
+
+            csunf comp; allsimpl.
+            apply compute_step_catch_success in comp.
+            repndors; exrepnd; subst; allsimpl; ginv.
+
+            * csunf; simpl; auto.
+
+            * csunf; simpl; auto.
+              rewrite compute_step_catch_if_diff; auto.
+
+          + SSCase "Abs".
+
+            csunf comp; allsimpl.
+            remember (compute_step lib1 (oterm (Abs abs2) bts)) as c.
+            destruct c; allsimpl; ginv.
+            symmetry in Heqc.
+
+            pose proof (ind (oterm (Abs abs2) bts) (oterm (Abs abs2) bts) []) as q; clear ind.
+            repeat (autodimp q hyp); eauto 2 with slow.
+            apply q in Heqc; clear q; eauto 2 with slow.
+            csunf; simpl.
+            rewrite Heqc; auto.
+      }
+
+      {
+        csunf comp; allsimpl.
+        apply compute_step_fresh_success in comp; exrepnd; subst.
+        repndors; exrepnd; subst; ginv.
+
+        - csunf; simpl; boolvar; auto.
+
+        - rewrite compute_step_fresh_if_isvalue_like2; auto.
+
+        - fold (mk_fresh n t).
+          rewrite compute_step_fresh_if_isnoncan_like; auto.
+
+          remember (get_fresh_atom lib1 t) as a.
+          pose proof (get_fresh_atom_prop_and_lib lib1 t) as prop; rewrite <- Heqa in prop.
+          clear Heqa.
+
+          remember (get_fresh_atom lib2 t) as a'.
+          pose proof (get_fresh_atom_prop_and_lib lib2 t) as prop'; rewrite <- Heqa' in prop'.
+          clear Heqa'.
+
+          simpl.
+          unfsubst in comp2.
+
+          pose proof (compute_step_subst_utoken2 lib1 t x n a a') as w.
+          repeat (autodimp w hyp); eauto 2 with slow.
+
+          pose proof (ind t (subst t n (mk_utoken a')) [n]) as q; clear ind.
+          repeat (autodimp q hyp); eauto 2 with slow;[|].
+          { rewrite simple_osize_subst; eauto 2 with slow. }
+          fold_terms.
+          unfsubst in q.
+          allrw @fold_subst_aux.
+          apply q in w;[|eauto 4 with wf slow]; clear q.
+
+          unfsubst.
+          allrw @fold_subst_aux.
+          allrw; simpl.
+
+          rewrite subst_utokens_var_ren_utok; auto.
+
+          apply compute_step_preserves_utokens in comp2;[|eauto 3 with slow wf].
+          destruct (get_patom_deq o a a'); tcsp;[].
+          left.
+          introv i; eapply get_utokens_subset_get_utokens_lib in i.
+          apply comp2 in i.
+          apply implies_get_utokens_lib_subst_aux2 in i; tcsp; eauto 2 with slow.
+      }
+
+    + SCase "Exc".
+
+      csunf comp; allsimpl; ginv.
+
+    + SCase "Abs".
+
+      csunf comp; allsimpl.
+      apply compute_step_lib_success in comp.
+      exrepnd; subst.
+
+      csunf; simpl.
+
+      apply (found_entry_implies_compute_step_lib_success _ _ _ _ _ _ correct).
+      eapply lib_extends_preserves_find_entry; eauto.
+Qed.
+
+Lemma lib_extends_preserves_reduces_in_atmost_k_steps {o} :
+  forall (lib1 lib2 : library)
+         (ext  : lib_extends lib2 lib1) (* lib2 extends lib1 *)
+         (a b  : @NTerm o)
+         (wfa  : wf_term a)
+         (n    : nat)
+         (comp : reduces_in_atmost_k_steps lib1 a b n),
+    reduces_in_atmost_k_steps lib2 a b n.
+Proof.
+  introv ext wf comp.
+
+  revert dependent a.
+  induction n; introv wf comp.
+
+  - allrw @reduces_in_atmost_k_steps_0; subst; auto.
+
+  - allrw @reduces_in_atmost_k_steps_S; exrepnd.
+    applydup @compute_step_preserves_wf in comp1; auto.
+    apply IHn in comp0; exrepnd; auto; clear IHn.
+    apply (lib_extends_preserves_compute_step lib1 lib2) in comp1; eauto 2 with slow.
+    allrw.
+    eexists; dands; eauto.
+Qed.
+
+Lemma lib_extends_preserves_reduces_to {o} :
+  forall (lib1 lib2 : library)
+         (ext  : lib_extends lib2 lib1) (* lib2 extends lib1 *)
+         (a b  : @NTerm o)
+         (wf   : wf_term a)
+         (comp : reduces_to lib1 a b),
+    reduces_to lib2 a b.
+Proof.
+  introv ext wf r.
+  unfold reduces_to in *; exrepnd.
+  eapply lib_extends_preserves_reduces_in_atmost_k_steps in r0; eauto.
+Qed.
+
+Lemma lib_extends_preserves_computes_to_value {o} :
+  forall (lib1 lib2 : library)
+         (ext  : lib_extends lib2 lib1) (* lib2 extends lib1 *)
+         (a b  : @NTerm o)
+         (wf   : wf_term a)
+         (comp : computes_to_value lib1 a b),
+    computes_to_value lib2 a b.
+Proof.
+  introv ext wf r.
+  unfold computes_to_value in *; repnd.
+  dup r0 as comp.
+  eapply lib_extends_preserves_reduces_to in r0;[|eauto|]; eauto 2 with slow.
+Qed.
